wip

Logic/Modal/Standard/Kripke/Grz/Definability.lean
@@ -1,125 +1,68 @@
 import Logic.Modal.Standard.Kripke.Geach
 
-def irreflexivize (R : α → α → Prop) := λ x y => x ≠ y ∧ R x y
-postfix:max "⁻ʳ" => irreflexivize
-
-abbrev WeaklyConverseWellFounded (R : α → α → Prop) := ConverseWellFounded R⁻ʳ
-
--- TODO: move?
-lemma dependent_choice
-  {R : α → α → Prop} (h : ∃ s : Set α, s.Nonempty ∧ ∀ a ∈ s, ∃ b ∈ s, R a b)
-  : ∃ f : ℕ → α, ∀ x, R (f x) (f (x + 1))
-  := by
-  obtain ⟨s, ⟨x, hx⟩, h'⟩ := h;
-  choose! f hfs hR using h';
-  use fun n ↦ f^[n] x;
-  intro n;
-  simp only [Function.iterate_succ'];
-  refine hR (f^[n] x) ?a;
-  induction n with
-  | zero => simpa;
-  | succ n ih => simp only [Function.iterate_succ']; apply hfs _ ih;
-
-lemma antisymm_of_WCWF : WeaklyConverseWellFounded R → Antisymmetric R := by
-  contrapose;
-  simp [Antisymmetric];
-  intro x y Rxy Ryz hxy;
-  apply ConverseWellFounded.iff_has_max.not.mpr;
-  push_neg;
-  use {x, y};
-  constructor;
-  . simp;
-  . intro z hz;
-    by_cases z = x;
-    . use y; simp_all [irreflexivize];
-    . use x; simp_all [irreflexivize];
-
--- TODO: move?
-lemma Finite.exists_ne_map_eq_of_infinite_lt {α β} [LinearOrder α] [Infinite α] [Finite β] (f : α → β)
-  : ∃ x y : α, (x < y) ∧ f x = f y
-  := by
-    obtain ⟨i, j, hij, e⟩ := Finite.exists_ne_map_eq_of_infinite f;
-    rcases lt_trichotomy i j with (hij | _ | hij);
-    . use i, j;
-    . contradiction;
-    . use j, i; simp [hij, e];
-
-lemma WCWF_of_antisymm_trans
-  {R : α → α → Prop}
-  (hFin : Finite α) (R_trans : Transitive R)
-  : Antisymmetric R → WeaklyConverseWellFounded R := by
-  contrapose;
-  intro hWCWF;
-  replace hWCWF := ConverseWellFounded.iff_has_max.not.mp hWCWF;
-  push_neg at hWCWF;
-  obtain ⟨f, hf⟩ := dependent_choice hWCWF; clear hWCWF;
-  simp [irreflexivize] at hf;
-
-  simp [Antisymmetric];
-  obtain ⟨i, j, hij, e⟩ := Finite.exists_ne_map_eq_of_infinite_lt f;
-  use (f i), (f (i + 1));
-  have ⟨hi₁, hi₂⟩ := hf i;
-  refine ⟨(by assumption), ?_, (by assumption)⟩;
-
-  have : i + 1 < j := lt_iff_le_and_ne.mpr ⟨by omega, by aesop⟩;
-  have H : ∀ i j, i < j → R (f i) (f j) := by
-    intro i j hij
-    induction hij with
-    | refl => exact hf i |>.2;
-    | step _ ih => exact R_trans ih $ hf _ |>.2;
-  have := H (i + 1) j this;
-  simpa [e];
-
 namespace LO.Modal.Standard
 
 namespace Kripke
 
+open LO.Kripke
 open System
 open Kripke
 open Formula (atom)
 open Formula.Kripke
+open Relation (IrreflGen)
 
 variable {α : Type u} [Inhabited α] [DecidableEq α]
 variable {F : Kripke.Frame}
 
-lemma axiomT_defines : AxiomSet.DefinesKripkeFrameClass (α := α) 𝗧 (ReflexiveFrameClass) := by
-  have := @axiomGeach_defines (α := α) _ (t := ⟨0, 0, 1, 0⟩);
-  simp [AxiomSet.Geach.T_def, GeachConfluentFrameClass] at this;
-  apply this;
+lemma axiomT_defines : ∀ {F : Frame}, (F#α ⊧* 𝗧 ↔ F ∈ ReflexiveFrameClass) := by
+  intro F;
+  have := @axiomGeach_defines (α := α) _ (t := ⟨0, 0, 1, 0⟩) (F := F);
+  simp [AxiomSet.Geach.T_def, GeachConfluentFrameClass, GeachConfluent] at this;
+  simp [Semantics.RealizeSet];
+  constructor;
+  . intro h x; exact this.mp h;
+  . intro h; exact this.mpr (by apply h);
 
-lemma axiomFour_defines : AxiomSet.DefinesKripkeFrameClass (α := α) 𝟰 (TransitiveFrameClass) := by
-  have := @axiomGeach_defines (α := α) _ (t := ⟨0, 2, 1, 0⟩);
-  simp [AxiomSet.Geach.Four_def, GeachConfluentFrameClass] at this;
-  apply this;
+lemma axiomFour_defines : ∀ {F : Frame}, (F#α ⊧* 𝟰 ↔ F ∈ TransitiveFrameClass) := by
+  intro F;
+  have := @axiomGeach_defines (α := α) _ (t := ⟨0, 2, 1, 0⟩) (F := F);
+  simp [AxiomSet.Geach.Four_def, GeachConfluentFrameClass, GeachConfluent] at this;
+  simp [Semantics.RealizeSet];
+  constructor;
+  . intro h x y z Rxy Ryz;
+    exact this.mp (by assumption) rfl _ Rxy Ryz;
+  . intro h;
+    apply this.mpr;
+    rintro x _ z rfl y Rxy Ryz;
+    exact h Rxy Ryz;
 
-
-private lemma valid_on_frame_T_and_Four_of_Grz (h : F# ⊧* (𝗚𝗿𝘇 : AxiomSet α)) : F# ⊧* ({□p ⟶ (p ⋏ (□p ⟶ □□p)) | (p : Formula α)}) := by
+private lemma valid_on_frame_T_and_Four_of_Grz (h : F#α ⊧* (𝗚𝗿𝘇 : AxiomSet α)) : F#α ⊧* ({□p ⟶ (p ⋏ (□p ⟶ □□p)) | (p : Formula α)}) := by
   simp_all [ValidOnFrame, ValidOnModel, Axioms.T, Axioms.Grz];
   intro p V x;
   let q := p ⋏ (□p ⟶ □□p);
-  have h₁ : Satisfies ⟨F#, V⟩ x (□p ⟶ □(□(q ⟶ □q) ⟶ q)) := K_sound.sound lemma_Grz₁! (by simp) V x;
-  have h₂ : Satisfies ⟨F#, V⟩ x (□(□(q ⟶ □q) ⟶ q) ⟶ q)  := h q V x;
+  have h₁ : Satisfies ⟨F#α, V⟩ x (□p ⟶ □(□(q ⟶ □q) ⟶ q)) := K_sound.sound lemma_Grz₁! (by simp) V x;
+  have h₂ : Satisfies ⟨F#α, V⟩ x (□(□(q ⟶ □q) ⟶ q) ⟶ q)  := h q V x;
   exact λ f => h₂ (h₁ f);
 
-private lemma valid_on_frame_T_of_Grz (h : F# ⊧* (𝗚𝗿𝘇 : AxiomSet α)) : F# ⊧* (𝗧 : AxiomSet α) := by
+private lemma valid_on_frame_T_of_Grz (h : F#α ⊧* (𝗚𝗿𝘇 : AxiomSet α)) : F#α ⊧* (𝗧 : AxiomSet α) := by
   have := valid_on_frame_T_and_Four_of_Grz h;
   simp_all [ValidOnFrame, ValidOnModel, Axioms.T, Axioms.Grz];
   intro p V x hx;
   exact Satisfies.and_def.mp (this p V x hx) |>.1
 
-private lemma valid_on_frame_Four_of_Grz (h : F# ⊧* (𝗚𝗿𝘇 : AxiomSet α)) : F# ⊧* (𝟰 : AxiomSet α) := by
+private lemma valid_on_frame_Four_of_Grz (h : F#α ⊧* (𝗚𝗿𝘇 : AxiomSet α)) : F#α ⊧* (𝟰 : AxiomSet α) := by
   have := valid_on_frame_T_and_Four_of_Grz h;
   simp_all [ValidOnFrame, ValidOnModel, Axioms.T, Axioms.Grz];
   intro p V x hx;
   exact (Satisfies.and_def.mp (this p V x hx) |>.2) hx;
 
-private lemma refl_of_Grz (h : F# ⊧* (𝗚𝗿𝘇 : AxiomSet α)) : Reflexive F := by
+private lemma refl_of_Grz (h : F#α ⊧* (𝗚𝗿𝘇 : AxiomSet α)) : Reflexive F := by
   exact axiomT_defines.mp $ (valid_on_frame_T_of_Grz h);
 
-private lemma trans_of_Grz (h : F# ⊧* (𝗚𝗿𝘇 : AxiomSet α)) : Transitive F := by
+private lemma trans_of_Grz (h : F#α ⊧* (𝗚𝗿𝘇 : AxiomSet α)) : Transitive F := by
   exact axiomFour_defines.mp $ (valid_on_frame_Four_of_Grz h);
 
-private lemma wcwf_of_Grz (h : F# ⊧* (𝗚𝗿𝘇 : AxiomSet α)) : WeaklyConverseWellFounded F := by
+private lemma WCWF_of_Grz (h : F#α ⊧* (𝗚𝗿𝘇 : AxiomSet α)) : WCWF F := by
   have F_trans : Transitive F := trans_of_Grz h;
   have F_refl : Reflexive F := refl_of_Grz h;
 
@@ -130,7 +73,7 @@ private lemma wcwf_of_Grz (h : F# ⊧* (𝗚𝗿𝘇 : AxiomSet α)) : WeaklyCon
   replace hWCWF := ConverseWellFounded.iff_has_max.not.mp hWCWF;
   push_neg at hWCWF;
   obtain ⟨f, hf⟩ := dependent_choice hWCWF; clear hWCWF;
-  simp [irreflexivize] at hf;
+  simp [IrreflGen] at hf;
 
   apply iff_not_validOnFrame.mpr;
   use (Axioms.Grz (atom default));
@@ -187,7 +130,7 @@ private lemma wcwf_of_Grz (h : F# ⊧* (𝗚𝗿𝘇 : AxiomSet α)) : WeaklyCon
         exact this _ hx;
       . simp [Satisfies, V];
 
-private lemma Grz_of_wcwf : (Reflexive F.Rel ∧ Transitive F.Rel ∧ WeaklyConverseWellFounded F.Rel) → F# ⊧* (𝗚𝗿𝘇 : AxiomSet α) := by
+private lemma Grz_of_wcwf : (Reflexive F.Rel ∧ Transitive F.Rel ∧ WeaklyConverseWellFounded F.Rel) → F#α ⊧* (𝗚𝗿𝘇 : AxiomSet α) := by
   rintro ⟨hRefl, hTrans, hWCWF⟩;
   simp [Axioms.Grz];
   intro p V;
@@ -196,7 +139,7 @@ private lemma Grz_of_wcwf : (Reflexive F.Rel ∧ Transitive F.Rel ∧ WeaklyConv
   let Y := { x | Satisfies ⟨F, V⟩ x (□(□(p ⟶ □p) ⟶ p)) ∧ ¬(Satisfies ⟨F, V⟩ x (□p)) ∧ (Satisfies ⟨F, V⟩ x p) };
   have : (X ∩ Y) = ∅ := by aesop;
 
-  suffices ∀ x ∈ X ∪ Y, ∃ y ∈ X ∪ Y, F.Rel⁻ʳ x y by
+  suffices ∀ x ∈ X ∪ Y, ∃ y ∈ X ∪ Y, (IrreflGen F.Rel) x y by
     have : (X ∪ Y) = ∅ := by
       by_contra hC;
       replace hC := Set.nonempty_iff_ne_empty.mpr hC;
