Logic/Vorspiel/BinaryRelations.lean
@@ -6,24 +6,24 @@ section
 variable {α : Type u} (rel : α → α → Prop)
 local infix:50 " ≺ " => rel
 
--- NOTE: `w₁ ≺ w₂ → w₁ ≺ w₃ → w₂ ≺ w₃`とする流儀もある
-def Euclidean := ∀ ⦃w₁ w₂ w₃⦄, w₁ ≺ w₂ → w₁ ≺ w₃ → w₃ ≺ w₂
+-- NOTE: `x ≺ y → x ≺ z → y ≺ z`とする流儀もある
+def Euclidean := ∀ ⦃x y z⦄, x ≺ y → x ≺ z → z ≺ y
 
-def Serial := ∀ w₁, ∃ w₂, w₁ ≺ w₂
+def Serial := ∀ x, ∃ y, x ≺ y
 
 def Confluent := ∀ ⦃x y z⦄, ((x ≺ y ∧ x ≺ z) → ∃ w, (y ≺ w ∧ z ≺ w))
 
-def Dense := ∀ ⦃w₁ w₂⦄, w₁ ≺ w₂ → ∃w₃, w₁ ≺ w₃ ∧ w₃ ≺ w₂
+def Dense := ∀ ⦃x y⦄, x ≺ y → ∃z, x ≺ z ∧ z ≺ y
 
 def Connected := ∀ ⦃x y z⦄, x ≺ y ∧ x ≺ z → y ≺ z ∨ z ≺ y
 
-def Functional := ∀ ⦃w₁ w₂ w₃⦄, w₁ ≺ w₂ ∧ w₁ ≺ w₃ → w₂ = w₃
+def Functional := ∀ ⦃x y z⦄, x ≺ y ∧ x ≺ z → y = z
 
-def RightConvergent := ∀ ⦃w₁ w₂ w₃⦄, w₁ ≺ w₂ ∧ w₁ ≺ w₃ → w₂ ≺ w₃ ∨ w₃ ≺ w₂ ∨ w₂ = w₃
+def RightConvergent := ∀ ⦃x y z⦄, x ≺ y ∧ x ≺ z → y ≺ z ∨ z ≺ y ∨ y = z
 
 def Extensive := ∀ ⦃x y⦄, x ≺ y → x = y
 
-def Antisymmetric := ∀ ⦃w₁ w₂⦄, w₁ ≺ w₂ → w₂ ≺ w₁ → w₁ = w₂
+def Antisymmetric := ∀ ⦃x y⦄, x ≺ y → y ≺ x → x = y
 
 def Isolated := ∀ ⦃x y⦄, ¬(x ≺ y)
 
@@ -32,6 +32,7 @@ def Assymetric := ∀ ⦃x y⦄, (x ≺ y) → ¬(y ≺ x)
 def Universal := ∀ ⦃x y⦄, x ≺ y
 
 abbrev ConverseWellFounded := WellFounded $ flip (· ≺ ·)
+alias CWF := ConverseWellFounded
 
 end
 
@@ -53,19 +54,19 @@ lemma serial_of_refl : Serial rel := by
 
 -- B + 4 → 5
 lemma eucl_of_symm_trans : Euclidean rel := by
-  intro w₁ w₂ w₃ r₁₂ r₁₃;
-  have r₂₁ := hSymm r₁₂;
-  exact hSymm $ hTrans r₂₁ r₁₃;
+  intro x y z Rxy Rxz;
+  have Ryx := hSymm Rxy;
+  exact hSymm $ hTrans Ryx Rxz;
 
 -- B + 5 → 4
 lemma trans_of_symm_eucl : Transitive rel := by
-  rintro w₁ w₂ w₃ r₁₂ r₂₃;
-  exact hSymm $ hEucl (hSymm r₁₂) r₂₃;
+  rintro x y z Rxy Ryz;
+  exact hSymm $ hEucl (hSymm Rxy) Ryz;
 
 -- T + 5 → B
 lemma symm_of_refl_eucl : Symmetric rel := by
-  intro w₁ w₂ r₁₂;
-  exact hEucl (hRefl w₁) r₁₂;
+  intro x y Rxy;
+  exact hEucl (hRefl x) Rxy;
 
 -- T + 5 → 4
 lemma trans_of_refl_eucl : Transitive rel := by
@@ -74,10 +75,10 @@ lemma trans_of_refl_eucl : Transitive rel := by
 
 -- B + D + 5 → T
 lemma refl_of_symm_serial_eucl : Reflexive rel := by
-  rintro w₁;
-  obtain ⟨w₂, r₁₂⟩ := hSerial w₁;
-  have r₂₁ := hSymm r₁₂;
-  exact trans_of_symm_eucl hSymm hEucl r₁₂ r₂₁;
+  rintro x;
+  obtain ⟨y, Rxy⟩ := hSerial x;
+  have Ryx := hSymm Rxy;
+  exact trans_of_symm_eucl hSymm hEucl Rxy Ryx;
 
 
 section ConverseWellFounded
@@ -115,5 +116,75 @@ lemma refl_of_universal (h : Universal rel) : Reflexive rel := by
 
 lemma eucl_of_universal (h : Universal rel) : Euclidean rel := by
   rintro x y z _ _; exact @h z y;
+
+
+
+def Relation.IrreflGen (R : α → α → Prop) := λ x y => x ≠ y ∧ R x y
+
+abbrev WeaklyConverseWellFounded (R : α → α → Prop) := CWF (Relation.IrreflGen R)
+alias WCWF := WeaklyConverseWellFounded
+
+section
+
+lemma dependent_choice {R : α → α → Prop} (h : ∃ s : Set α, s.Nonempty ∧ ∀ a ∈ s, ∃ b ∈ s, R a b)
+  : ∃ f : ℕ → α, ∀ x, R (f x) (f (x + 1)) := by
+  obtain ⟨s, ⟨x, hx⟩, h'⟩ := h;
+  choose! f hfs hR using h';
+  use fun n ↦ f^[n] x;
+  intro n;
+  simp only [Function.iterate_succ'];
+  refine hR (f^[n] x) ?a;
+  induction n with
+  | zero => simpa;
+  | succ n ih => simp only [Function.iterate_succ']; apply hfs _ ih;
+
+lemma Finite.exists_ne_map_eq_of_infinite_lt {α β} [LinearOrder α] [Infinite α] [Finite β] (f : α → β)
+  : ∃ x y : α, (x < y) ∧ f x = f y
+  := by
+    obtain ⟨i, j, hij, e⟩ := Finite.exists_ne_map_eq_of_infinite f;
+    rcases lt_trichotomy i j with (hij | _ | hij);
+    . use i, j;
+    . contradiction;
+    . use j, i; simp [hij, e];
+
+lemma antisymm_of_WCWF {R : α → α → Prop} : WCWF R → Antisymmetric R := by
+  contrapose;
+  simp [Antisymmetric];
+  intro x y Rxy Ryz hxy;
+  apply ConverseWellFounded.iff_has_max.not.mpr;
+  push_neg;
+  use {x, y};
+  constructor;
+  . simp;
+  . intro z hz;
+    by_cases z = x;
+    . use y; simp_all [Relation.IrreflGen];
+    . use x; simp_all [Relation.IrreflGen];
+
+lemma WCWF_of_finite_trans_antisymm {R : α → α → Prop} (hFin : Finite α) (R_trans : Transitive R)
+  : Antisymmetric R → WCWF R := by
+    contrapose;
+    intro hWCWF;
+    replace hWCWF := ConverseWellFounded.iff_has_max.not.mp hWCWF;
+    push_neg at hWCWF;
+    obtain ⟨f, hf⟩ := dependent_choice hWCWF; clear hWCWF;
+    simp [Relation.IrreflGen] at hf;
+
+    simp [Antisymmetric];
+    obtain ⟨i, j, hij, e⟩ := Finite.exists_ne_map_eq_of_infinite_lt f;
+    use (f i), (f (i + 1));
+    have ⟨hi₁, hi₂⟩ := hf i;
+    refine ⟨(by assumption), ?_, (by assumption)⟩;
+
+    have : i + 1 < j := lt_iff_le_and_ne.mpr ⟨by omega, by aesop⟩;
+    have H : ∀ i j, i < j → R (f i) (f j) := by
+      intro i j hij
+      induction hij with
+      | refl => exact hf i |>.2;
+      | step _ ih => exact R_trans ih $ hf _ |>.2;
+    have := H (i + 1) j this;
+    simpa [e];
+
+end
 
 end
